LeanYjs/ItemSet.lean
@@ -1,3 +1,213 @@
 import LeanYjs.Item
+import LeanYjs.ItemOriginOrder
+import LeanYjs.ActorId
+import LeanYjs.ItemOrder
+
+import Mathlib.Tactic.Set
+
+variable {A : Type} [BEq A]
+
+-- Defines a subset of YjsItem which are possible DAG of a history of insertions.
+
+variable (P : ClosedPredicate A)
+
+def ItemSet := { i : YjsItem A // P.val i }
+
+def OriginLeq' (x y : ItemSet P) : Prop :=
+  x = y ∨ OriginLt A P (↑x.1) (↑y.1)
+
+def YjsLt' (x y : ItemSet P) : Prop :=
+  ∃ h, @YjsLt A P h (↑x.1) (↑y.1)
+
+def YjsLeq' (x y : ItemSet P) : Prop :=
+  ∃ h, @YjsLeq A P h (↑x.1) (↑y.1)
+
+def YjsInvariant :=
+  forall h (x y : YjsItem A),
+    P.val x -> P.val y ->
+    @YjsLt A P h x y ->
+      (∃ h, @YjsLeq A P h x (y.origin)) ∨
+      (∃ h,  @YjsLt A P h (y.origin) (x.origin)) ∨
+      (x.origin = y.origin ∧ ((∃ h, @YjsLt A P h x.rightOrigin y) ∨ x.id < y.id))
+
+def ItemSetInvariant :=
+  P.val YjsPtr.first ∧
+  P.val YjsPtr.last ∧
+  (∀ (o : YjsPtr A) r id c, P.val (YjsItem.item o r id c) -> P.val o) ∧
+  (∀ o (r : YjsPtr A) id c, P.val (YjsItem.item o r id c) -> P.val r) ∧
+  (∀ (x y : YjsPtr A), P.val x -> P.val y -> OriginLt A P x y -> OriginLt A P y x -> False) ∧
+  YjsInvariant P
+
+lemma origin_p_valid {A} {P : ClosedPredicate A} : forall (x : YjsItem A), P.val x -> P.val x.origin := by
+  intros x px
+  obtain ⟨ p, ⟨ hp, hp', hp'', hp''' ⟩ ⟩ := P
+  simp at *
+  obtain ⟨ o, r, id, c ⟩ := x
+  simp [YjsItem.origin] at *
+  tauto
+
+lemma right_origin_p_valid {A} {P : ClosedPredicate A} : forall (x : YjsItem A), P.val x -> P.val x.rightOrigin := by
+  intros x px
+  obtain ⟨ p, ⟨ hp, hp', hp'', hp''' ⟩ ⟩ := P
+  simp at *
+  obtain ⟨ o, r, id, c ⟩ := x
+  simp [YjsItem.rightOrigin] at *
+  tauto
 
 
+lemma not_item_lt_first {A} {P : ClosedPredicate A} : ItemSetInvariant P -> ∀ h (o : YjsItem A), ¬ @YjsLt A P h o YjsPtr.first := by
+  intros hinv h o
+  apply @Nat.strongRecOn' (P := fun h => ∀ (o : YjsItem A), ¬ @YjsLt A P h o YjsPtr.first)
+  intros n ih o hlt
+  cases hlt with
+  | ltConflict h _ _ hlt =>
+    cases hlt
+  | ltOriginOrder _ _ hlt =>
+    have hlt2 : @OriginLt A P YjsPtr.first o := by
+      apply OriginLt.ltOrigin (x := YjsPtr.first) (y := YjsPtr.itemPtr o)
+      . apply hinv.1
+      . apply origin_lt_p1 at hlt; assumption
+      . apply OriginLtStep.lt_first
+    obtain ⟨ hfirst, hlast, hleft, hright, hanti, hinv ⟩ := hinv
+    apply hanti (x := YjsPtr.first) (y := o) <;> try assumption
+    apply origin_lt_p1 at hlt; assumption
+  | ltTrans h1 h2 x y z hlt1 hlt2 =>
+    have hlt_h2 : h2 < max h1 h2 + 1 := by
+      omega
+    apply ih _ hlt_h2 _ hlt2
+
+lemma not_last_lt_item {A} {P : ClosedPredicate A} : ItemSetInvariant P -> ∀ h (o : YjsItem A), ¬ @YjsLt A P h YjsPtr.last o := by
+  intros hinv h o
+  apply @Nat.strongRecOn' (P := fun h => ∀ (o : YjsItem A), ¬ @YjsLt A P h YjsPtr.last o)
+  intros n ih o hlt
+  cases hlt with
+  | ltConflict h _ _ hlt =>
+    cases hlt
+  | ltOriginOrder _ _ hlt =>
+    have hlt2 : @OriginLt A P o YjsPtr.last := by
+      apply OriginLt.ltOrigin (x := YjsPtr.itemPtr o) (y := YjsPtr.last)
+      . apply origin_lt_p2 at hlt; assumption
+      . apply hinv.2.1
+      . apply OriginLtStep.lt_last
+    obtain ⟨ hfirst, hlast, hleft, hright, hanti, hinv ⟩ := hinv
+    apply hanti (x := YjsPtr.last) (y := o) <;> try assumption
+    apply origin_lt_p2 at hlt; assumption
+  | ltTrans h1 h2 x y z hlt1 hlt2 =>
+    have hlt_h2 : h1 < max h1 h2 + 1 := by
+      omega
+    apply ih _ hlt_h2 _ hlt1
+
+lemma not_last_lt_first {A} {P : ClosedPredicate A} : ItemSetInvariant P -> ∀ h, ¬ @YjsLt A P h YjsPtr.last YjsPtr.first := by
+  intros hinv h
+  apply @Nat.strongRecOn' (P := fun h => ¬ @YjsLt A P h YjsPtr.last YjsPtr.first)
+  intros n ih hlt
+  cases hlt with
+  | ltConflict h _ _ hlt =>
+    cases hlt
+  | ltOriginOrder _ _ hlt =>
+    have hlt' : OriginLt _ P YjsPtr.first YjsPtr.last := by
+      obtain ⟨ P, ⟨ a, b, c ⟩ ⟩ := P
+      apply OriginLt.ltOrigin <;> try assumption
+      apply OriginLtStep.lt_first_last
+    obtain ⟨ hfirst, hlast, hleft, hright, hanti, hinv ⟩ := hinv
+    apply hanti (x := YjsPtr.first) (y := YjsPtr.last) <;> assumption
+  | ltTrans h1 h2 x y z hlt1 hlt2 =>
+    apply not_item_lt_first at hlt2 <;> assumption
+
+lemma not_first_lt_first {A} {P : ClosedPredicate A} : ItemSetInvariant P -> ∀ h, ¬ @YjsLt A P h YjsPtr.first YjsPtr.first := by
+  intros hinv h hlt
+  have h: OriginLt A P YjsPtr.first YjsPtr.first := by
+    cases hlt with
+    | ltConflict h _ _ hlt =>
+      cases hlt
+    | ltTrans h1 h2 x y z hlt1 hlt2 =>
+      apply not_item_lt_first hinv at hlt2; contradiction
+    | ltOriginOrder _ _ hlt =>
+      assumption
+  obtain ⟨ hfirst, hlast, hleft, hright, hanti, hinv ⟩ := hinv
+  apply hanti (x := YjsPtr.first) (y := YjsPtr.first) <;> try assumption
+
+lemma not_last_lt_last {A} {P : ClosedPredicate A} : ItemSetInvariant P -> ∀ h, ¬ @YjsLt A P h YjsPtr.last YjsPtr.last := by
+  intros hinv h hlt
+  have h: OriginLt A P YjsPtr.last YjsPtr.last := by
+    cases hlt with
+    | ltConflict h _ _ hlt =>
+      cases hlt
+    | ltTrans h1 h2 x y z hlt1 hlt2 =>
+      apply not_last_lt_item hinv at hlt1; contradiction
+    | ltOriginOrder _ _ hlt =>
+      assumption
+  obtain ⟨ hfirst, hlast, hleft, hright, hanti, hinv ⟩ := hinv
+  apply hanti (x := YjsPtr.last) (y := YjsPtr.last) <;> try assumption
+
+lemma not_ptr_lt_first {A} {P : ClosedPredicate A} : ItemSetInvariant P -> ∀ h (o : YjsPtr A), ¬ @YjsLt A P h o YjsPtr.first := by
+  intros hinv h o
+  cases o with
+  | itemPtr item =>
+    apply not_item_lt_first hinv
+  | first =>
+    apply not_first_lt_first hinv
+  | last =>
+    apply not_last_lt_first hinv
+
+lemma not_last_lt_ptr {A} {P : ClosedPredicate A} : ItemSetInvariant P -> ∀ h (o : YjsPtr A), ¬ @YjsLt A P h YjsPtr.last o := by
+  intros hinv h o
+  cases o with
+  | itemPtr item =>
+    apply not_last_lt_item hinv
+  | first =>
+    apply not_last_lt_first hinv
+  | last =>
+    apply not_last_lt_last hinv
+
+lemma yjs_lt_p_trans {A} {P : ClosedPredicate A} (inv : ItemSetInvariant P) (x y z : YjsPtr A) h1 h2:
+  @YjsLt A P h1 x y -> @YjsLt A P h2 y z -> @YjsLt A P (max h1 h2 + 1) x z := by
+  intros hlt1 hlt2
+  cases y with
+  | first =>
+    apply not_ptr_lt_first inv at hlt1; contradiction
+  | last =>
+    apply not_last_lt_ptr inv at hlt2; contradiction
+  | itemPtr y =>
+    apply YjsLt.ltTrans <;> assumption
+
+lemma yjs_leq_p_trans1 {A} {P : ClosedPredicate A} (inv : ItemSetInvariant P) (x y z : YjsPtr A) h1 h2:
+  @YjsLeq A P h1 x y -> @YjsLt A P h2 y z -> ∃ h, @YjsLt A P h x z := by
+  intros hleq hlt
+  cases hleq with
+  | inl heq =>
+    rw [heq]
+    exists h2
+  | inr hlt =>
+    exists (max h1 h2 + 1)
+    apply yjs_lt_p_trans <;> assumption
+
+lemma yjs_leq_p_trans2 {A} {P : ClosedPredicate A} (inv : ItemSetInvariant P) (x y z : YjsPtr A) h1 h2:
+  @YjsLt A P h1 x y -> @YjsLeq A P h2 y z -> ∃ h, @YjsLt A P h x z := by
+  intros hlt hleq
+  cases hleq with
+  | inl heq =>
+    rw [<-heq]
+    exists h1
+  | inr hlt =>
+    exists (max h1 h2 + 1)
+    apply yjs_lt_p_trans <;> assumption
+
+lemma yjs_leq_p_trans {A} {P : ClosedPredicate A} (inv : ItemSetInvariant P) (x y z : YjsPtr A) h1 h2:
+  @YjsLeq A P h1 x y -> @YjsLeq A P h2 y z -> ∃ h, @YjsLeq A P h x z := by
+  intros hleq1 hleq2
+  cases hleq1 with
+  | inl heq =>
+    rw [heq]
+    exists h2
+  | inr hlt =>
+    cases hleq2 with
+    | inl heq =>
+      rw [<-heq]
+      exists h1
+      right
+      assumption
+    | inr hlt =>
+      exists (max h1 h2 + 1)
+      right
+      apply yjs_lt_p_trans <;> assumption
