LeanYjs/Totality.lean
@@ -1,0 +1,173 @@
+import LeanYjs.Item
+import LeanYjs.ActorId
+import LeanYjs.ItemOriginOrder
+import LeanYjs.ItemOrder
+import LeanYjs.ItemSet
+
+@[simp] lemma first_p_valid {A} {P : ClosedPredicate A} : P.val YjsPtr.first := by
+  unfold ClosedPredicate at *
+  obtain ⟨ p, ⟨ hp, hp', hp'', hp''' ⟩ ⟩ := P
+  assumption
+
+@[simp] lemma last_p_valid {A} {P : ClosedPredicate A} : P.val YjsPtr.last := by
+  unfold ClosedPredicate at *
+  obtain ⟨ p, ⟨ hp, hp', hp'', hp''' ⟩ ⟩ := P
+  assumption
+
+lemma yjs_lt_total {A : Type} {P : @ClosedPredicate A} {inv : ItemSetInvariant P} {x y : YjsPtr A} (hx : P.val x) (hy : P.val y) :
+  (∃ h, @YjsLeq A P h x y) ∨ (∃ h, @YjsLt A P h y x) :=
+  match x with
+  | YjsPtr.first =>
+    match y with
+    | YjsPtr.first => by
+      left
+      exists 0
+      left
+      simp
+    | YjsPtr.last => by
+      left
+      exists 0
+      right
+      apply YjsLt.ltOriginOrder
+      apply OriginLt.ltOrigin <;> try simp
+      apply OriginLtStep.lt_first_last
+    | YjsPtr.itemPtr item => by
+      left
+      exists 0
+      right
+      apply YjsLt.ltOriginOrder
+      apply OriginLt.ltOrigin <;> try first | simp | assumption
+      apply OriginLtStep.lt_first
+  | YjsPtr.last =>
+    match y with
+    | YjsPtr.first => by
+      right
+      exists 0
+      apply YjsLt.ltOriginOrder
+      apply OriginLt.ltOrigin <;> try first | simp | assumption
+      apply OriginLtStep.lt_first_last
+    | YjsPtr.last => by
+      left
+      exists 0
+      left
+      simp
+    | YjsPtr.itemPtr item => by
+      right
+      exists 0
+      apply YjsLt.ltOriginOrder
+      apply OriginLt.ltOrigin <;> try first | simp | assumption
+      apply OriginLtStep.lt_last
+  | YjsPtr.itemPtr x =>
+    match y with
+    | YjsPtr.first => by
+      right
+      exists 0
+      apply YjsLt.ltOriginOrder
+      apply OriginLt.ltOrigin <;> try first | simp | assumption
+      apply OriginLtStep.lt_first
+    | YjsPtr.last => by
+      left
+      exists 0
+      right
+      apply YjsLt.ltOriginOrder
+      apply OriginLt.ltOrigin <;> try first | simp | assumption
+      apply OriginLtStep.lt_last
+    | YjsPtr.itemPtr y => by
+      obtain ⟨ xo, xr, xid, xc ⟩ := x
+      obtain ⟨ yo, yr, yid, yc ⟩ := y
+      have hxo : P.val xo := by
+        apply origin_p_valid (YjsItem.item xo xr xid xc) hx
+      have hyo : P.val yo := by
+        apply origin_p_valid (YjsItem.item yo yr yid yc) hy
+      have hxr : P.val xr := by
+        apply right_origin_p_valid (YjsItem.item xo xr xid xc) hx
+      have hyr : P.val yr := by
+        apply right_origin_p_valid (YjsItem.item yo yr yid yc) hy
+      obtain hleq := yjs_lt_total hx hyo
+      cases hleq with
+      | inl hleq =>
+        obtain ⟨ h, hleq ⟩ := hleq
+        left
+        suffices (∃ h, YjsLt P h (YjsPtr.itemPtr (YjsItem.item xo xr xid xc)) (YjsPtr.itemPtr (YjsItem.item yo yr yid yc))) from by
+          obtain ⟨ h, hlt ⟩ := this
+          exists h
+          right
+          assumption
+        apply yjs_leq_p_trans1 inv _ _ _ _ 0 hleq _
+        apply YjsLt.ltOriginOrder
+        apply OriginLt.ltOrigin <;> try first | simp | assumption
+        apply OriginLtStep.lt_left
+      | inr hltyox =>
+        obtain hleq := yjs_lt_total hyr hx
+        cases hleq with
+        | inl hleq =>
+          obtain ⟨ h, hleq ⟩ := hleq
+          right
+          apply yjs_leq_p_trans2 inv _ _ _ 0 _ _ hleq
+          apply YjsLt.ltOriginOrder
+          apply OriginLt.ltOrigin <;> try first | simp | assumption
+          apply OriginLtStep.lt_right
+        | inr hltxyr =>
+          obtain hleq := yjs_lt_total hy hxo
+          cases hleq with
+          | inl hleq =>
+            obtain ⟨ h, hleq ⟩ := hleq
+            right
+            apply yjs_leq_p_trans1 inv _ _ _ _ 0 hleq _
+            apply YjsLt.ltOriginOrder
+            apply OriginLt.ltOrigin <;> try first | simp | assumption
+            apply OriginLtStep.lt_left
+          | inr hltxoy =>
+            obtain hleq := yjs_lt_total hxr hy
+            cases hleq with
+            | inl hleq =>
+              obtain ⟨ h, hleq ⟩ := hleq
+              left
+              apply yjs_leq_p_trans inv _ _ _ 0 _ _ hleq
+              right
+              apply YjsLt.ltOriginOrder
+              apply OriginLt.ltOrigin <;> try first | simp | assumption
+              apply OriginLtStep.lt_right
+            | inr hltyxr =>
+              obtain ⟨ h1, hlt_yo_x ⟩ := hltyox
+              obtain ⟨ h2, hlt_x_yo ⟩ := hltxoy
+              obtain ⟨ h3, hlt_x_yr ⟩ := hltxyr
+              obtain ⟨ h4, hlt_y_xr ⟩ := hltyxr
+              obtain hleq := yjs_lt_total hxo hyo
+              cases hleq with
+              | inr hlt =>
+                obtain ⟨ h5, hlt_yo_xr ⟩ := hlt
+                left
+                exists (max4 h5 h3 h2 h4 + 1 + 1)
+                right
+                apply YjsLt.ltConflict
+                apply ConflictLt.ltOriginDiff <;> try first | simp | assumption
+              | inl hleq =>
+                obtain ⟨ h5, hlt_yo_xr ⟩ := hleq
+                cases hlt_yo_xr with
+                | inr hlt =>
+                  right
+                  exists (max4 h5 h4 h1 h3 + 1 + 1)
+                  apply YjsLt.ltConflict
+                  apply ConflictLt.ltOriginDiff <;> try first | simp | assumption
+                | inl heq =>
+                  rw [heq] at hlt_yo_x hlt_x_yo hlt_x_yr
+                  rw [heq]
+                  have hid : xid < yid ∨ yid < xid ∨ xid = yid := by
+                    unfold ActorId; omega
+                  cases hid with
+                  | inl hlt =>
+                    left
+                    exists max h3 h4 + 1 + 1
+                    right
+                    apply YjsLt.ltConflict
+                    apply ConflictLt.ltOriginSame <;> try assumption
+                  | inr hleq =>
+                    cases hleq with
+                    | inl hlt =>
+                      right
+                      exists max h4 h3 + 1 + 1
+                      apply YjsLt.ltConflict
+                      apply ConflictLt.ltOriginSame <;> try assumption
+                    | inr heq =>
+                      sorry
